Add trait specializations
Addresses my concern about needing to know the concrete types of Enumerators to prove behaviors

examples/Enumerators/Datatypes.dfy
@@ -9,90 +9,57 @@ module DatatypeEnumerator {
 
   import opened Enumerators
   
-  // TODO: A TreeEnumerator would be much more interesting!
-  // Show how to implement multiple traversal options, probably
-  // using ConcatEnumerator for child paths.
+  datatype Tree<T> = Node(left: Tree<T>, value: T, right: Tree<T>) | Nil
 
-  // TODO: Could define a Enumerable<T> trait as well, although datatypes
-  // can't yet implement that anyway.
-  datatype List<T> = Cons(value: T, tail: List<T>) | Nil {
+  datatype TreeTraversal<T> = InorderTraversal(Tree<T>) /* | PreorderTraversal(Tree<T>) | PostorderTraversal(Tree<T>) */ {
     method Enumerator() returns (e: Enumerator<T>) 
       ensures e.Valid()
       ensures fresh(e.Repr)
+      ensures e.enumerated == []
     {
-      e := new ListEnumerator(this);
+      match this
+      case InorderTraversal(tree) => {
+        e := InorderEnumerator(tree);
+      }
     }
   }
 
-  class ListEnumerator<T> extends Enumerator<T> {
-
-    var next: List<T>
-
-    constructor(next: List<T>) 
-      ensures Valid()
-      ensures fresh(Repr - {this})
-    {
-      this.next := next;
-
-      enumerated := [];
-      Repr := {this};
+  method InorderEnumerator<T>(tree: Tree<T>) returns (e: Enumerator<T>) 
+    ensures e.Valid()
+    ensures fresh(e.Repr)
+    ensures e.enumerated == []
+  {
+    match tree
+    case Nil => {
+      e := new SeqEnumerator([]);
     }
-
-    predicate Valid() 
-      reads this, Repr 
-      ensures Valid() ==> this in Repr 
-      decreases Repr, 0
-    {
-      && this in Repr
-    }
-
-    function Decreases(): nat
-      reads Repr
-      requires Valid()
-      decreases Repr, 1
-    {
-      // TODO: This is where I wish I could just say "next" and 
-      // rely on the well-founded ordering.
-      Length(next)
-    }
-
-
-    static function Length(l: List<T>): nat {
-      match l
-      case Cons(_, tail) => 1 + Length(tail)
-      case Nil => 0
-    }
-
-    predicate method HasNext() 
-      reads Repr
-      requires Valid()
-      decreases Repr, 2
-      ensures Decreases() == 0 ==> !HasNext()
-    {
-      next.Cons?
-    }
-
-    method Next() returns (element: T)
-      requires Valid()
-      requires HasNext()
-      modifies Repr
-      decreases Repr
-      ensures Valid()
-      ensures Repr <= old(Repr)
-      ensures Decreases() < old(Decreases())
-      ensures enumerated == old(enumerated) + [element]
-    {
-      element := next.value;
-      next := next.tail;
-
-      enumerated := enumerated + [element];
+    case Node(left, value, right) => {
+      // TODO: How to make this lazy?
+      var thisValueEnum := new SeqEnumerator([value]);
+      var leftEnum := InorderEnumerator(left);
+      var rightEnum := InorderEnumerator(right);
+      var tmp := new ConcatEnumerator(leftEnum, thisValueEnum);
+      e := new ConcatEnumerator(tmp, rightEnum);
     }
   }
 
   method Main() {
-    var list := Cons(1, Cons(2, Cons(3, Cons(4, Cons(5, Nil)))));
+    var tree := Node(
+      Node(
+        Nil, 
+        1, 
+        Node(Nil, 2, Nil)
+      ), 
+      3,
+      Node(
+        Node(Nil, 4, Nil),
+        5,
+        Nil
+      )
+    );
 
-    var e := list.Enumerator();
+    var traversal := InorderTraversal(tree);
+    var e := traversal.Enumerator();
     while e.HasNext()
       invariant e.Valid() && fresh(e.Repr)
       decreases e.Decreases()
@@ -101,5 +68,12 @@ module DatatypeEnumerator {
 
       print x;
     }
+
+    // With foreach loop support, the above could just be:
+    //
+    // foreach x in InorderTraversal(tree) {
+    //   print x; 
+    // }
+
   }
 }
